Hs/Metatheory/Preservation.lean
@@ -1,25 +1,46 @@
 import Hs.CompileJ
 
+@[simp]
+abbrev HsKindLike : HsTerm -> Term -> Prop
+| k1 `-k> k2 , k1' -k> k2' => HsKindLike k1 k1' ∧ HsKindLike k2 k2'
+| `★, ★ => true
+| _, _ => false
 
+@[simp]
+abbrev KindLike : Term -> Prop
+| _ -k> _ => true
+| ★ => true
+| _ => false
+
+@[simp]
+abbrev HsTypeLike (Γ : Ctx HsTerm) : HsTerm -> Prop
+| .HsBind2 .arrow _ _ => true
+| .HsBind2 .all _ _ => true
+| `# x => (Γ d@ x).is_datatype
+| _ => false
+
+
+-- needs some sort of classification lemma?
 @[simp]
 abbrev CompileCtxWfType : (v : CompileVariant) -> (Γ : Ctx HsTerm) -> (CompileJArgs v Γ) -> Prop
 | .term => λ Γ => λ ⟨t , τ ; j , t'⟩ => ∀ Γ' τ',
   CompileJ .ctx Γ Γ' ->
   CompileJ .term Γ ⟨t, τ; j, t'⟩ ->
   (jk : Γ ⊢s τ : `★) ->
-  CompileJ .type Γ ⟨τ, `★; jk, τ'⟩ ∧ (Γ' ⊢ t' : τ')
-| .type => λ Γ => λ ⟨τ , k ; j , τ'⟩ => ∀ Γ',
-  k = `★ ->
+  CompileJ .type Γ ⟨τ, `★; jk, τ'⟩ ->
+  (Γ' ⊢ t' : τ')
+| .type => λ Γ => λ ⟨τ , k ; j , τ'⟩ => ∀ Γ' k',
   CompileJ .ctx Γ Γ' ->
-  CompileJ .type Γ ⟨τ, k; j, τ'⟩ ->
+  HsKindLike k k' ->
   (jk : Γ ⊢s k : `□) ->
-  CompileJ .kind Γ ⟨k, `□; jk, ★⟩ ∧  (Γ' ⊢ τ' : ★)
+  CompileJ .kind Γ ⟨k, `□; jk, k'⟩ ->
+  CompileJ .type Γ ⟨τ, k; j, τ'⟩ ->
+  (Γ' ⊢ τ' : k')
 | .kind => λ Γ => λ ⟨k , ki ; j , k'⟩ => ∀ Γ',
   ki = `□ ->
   CompileJ .ctx Γ Γ' ->
   CompileJ .kind Γ ⟨k, ki; j, k'⟩ ->
   (Γ' ⊢ k' : □)
-
 | .ctx => λ Γ => λ Γ' => ⊢s Γ -> CompileJ .ctx Γ Γ' -> ⊢ Γ'
 
 theorem compile_preserves_validctors :
@@ -44,114 +65,108 @@ theorem compile_preserves_typing :
  CompileJ v Γ idx -> CompileCtxWfType v Γ idx :=
 by
 intro j; induction j <;> simp at *;
-all_goals try (intro wf cc; cases cc; cases wf)
-case _ => apply Judgment.wfnil
-case _ ih cc wf =>
+case _ => intro wf cc; apply Judgment.wfnil
+case _ ih =>
+  intro wf cc
+  cases cc; cases wf;
+  case _ cc wf =>
   apply Judgment.wfempty (ih wf cc);
-case _  Γ' j c1 c2 ih1 ih2 _ _ j1 wf _ =>
+case _  Γ' j c1 c2 ih1 ih2 =>
+  intro wf cc
+  cases cc; cases wf;
+  case _ cc wf _ =>
   apply Judgment.wftype;
-  have ih2' := ih2 Γ' c2 c1 (HsJudgment.ax wf);
-  cases ih2'; assumption
-  apply ih1 wf c2
-case _ Γ' j1 c1 c2 ih1 ih2 j2 c3 c4 wf j4 =>
+  have ih1' := ih1 Γ' ★ c2; simp at ih1';
+  have ih1'' := ih1' (HsJudgment.ax wf) (CompileJ.type wf cc) c1;
+  assumption
+  apply ih2 wf c2;
+case _ Γ' j1 c1 c2 ih1 ih2 =>
+  intro wf cc
+  cases cc; cases wf;
+  case _ cc wf _ =>
   apply Judgment.wfkind;
   apply ih2 Γ' c2 c1
   apply ih1 wf c2
-case _ Γ' j1 c1 c2 ih1 ih2 j2 c3 c4 wf j4 =>
+case _ Γ' j1 c1 c2 ih1 ih2 =>
+  intro wf cc
+  cases cc; cases wf;
+  case _ cc wf _ =>
   apply Judgment.wfdatatype
   apply ih2 Γ' c2 c1
   apply ih1 wf c2
-case _ Γ' j1 c1 c2 ih1 ih2 j2 c3 c4 wf j3 j4 =>
+case _ Γ' j1 c1 c2 ih1 ih2 =>
+  intro wf cc
+  cases cc; cases wf;
+  case _ cc wf _ j4 =>
   apply Judgment.wfctor;
-  have ih2' := ih2 Γ' c2 c1 (HsJudgment.ax wf);
-  cases ih2'; assumption;
-  apply ih1 wf c2
-  apply compile_preserves_validctors j1 j4 c2 c1
-case _ A' _ Γ' j1 j2 c1 c2 c3 ih1 ih2 ih3 j3 j4 c4 c5 c6 wf j5 j6 =>
+  have ih1' := ih1 Γ' ★; simp at ih1';
+  have ih1'' := ih1' cc (HsJudgment.ax wf) (CompileJ.type wf cc) c1;
+  assumption;
+  apply ih2 wf c2
+  apply compile_preserves_validctors j1 j4 c2 c1;
+case _ A' _ Γ' j1 j2 c1 c2 c3 ih1 ih2 ih3 =>
+  intro wf cc
+  cases cc; cases wf;
+  case _ cc wf _ _ =>
   apply Judgment.wfterm;
-  have ih3' := ih3 Γ' c3 c1 (HsJudgment.ax wf); cases ih3'; assumption
-  have ih1' := ih1 Γ' A' c3 c2 j1;
-  cases ih1'; assumption;
-  apply ih2 wf c3
-
-all_goals try (intro Γ' cc c1)
-case _ wf =>
+  have ih1' := ih1 Γ' ★; simp at ih1';
+  have ih1'' := ih1' cc (HsJudgment.ax wf) (CompileJ.type wf cc) c1; assumption
+  have ih2' := ih2 Γ' A' c3 c2 j1 c1; assumption;
+  apply ih3 wf c3
+case _ wf cc ih =>
+  intro Γ' cc cc'
+  apply Judgment.ax;
   sorry
-case _ => sorry
-case _ => sorry
-case _ => sorry
-case _ => sorry
-case _ => sorry
-case _ => sorry
-case _ => sorry
-case _ => sorry
-case _ => sorry
-case _ => sorry
-case _ => sorry
-case _ => sorry
-case _ => sorry
-case _ => sorry
-case _ => sorry
-case _ => sorry
-case _ => sorry
-case _ => sorry
-case _ => sorry
-case _ => sorry
-case _ => sorry
-case _ => sorry
-case _ => sorry
-case _ => sorry
-case _ => sorry
-case _ => sorry
-case _ => sorry
-case _ => sorry
-case _ => sorry
-case _ => sorry
-case _ => sorry
-case _ => sorry
-case _ => sorry
-case _ => sorry
-case _ => sorry
-case _ => sorry
-case _ => sorry
-case _ => sorry
-case _ => sorry
-case _ => sorry
-case _ => sorry
-case _ => sorry
-case _ => sorry
-case _ => sorry
-case _ => sorry
-case _ => sorry
-case _ => sorry
-case _ => sorry
-case _ => sorry
-case _ => sorry
-case _ => sorry
-case _ => sorry
-case _ => sorry
-case _ => sorry
-case _ => sorry
-case _ => sorry
-case _ => sorry
-case _ => sorry
-case _ => sorry
-case _ => sorry
-case _ => sorry
-case _ => sorry
-case _ => sorry
-case _ => sorry
-case _ => sorry
-case _ => sorry
-case _ => sorry
-case _ => sorry
-case _ => sorry
-case _ => sorry
-case _ => sorry
-case _ => sorry
-case _ => sorry
-case _ => sorry
-case _ => sorry
+
+case _ j1 j2 j3 c1 c2 ih1 ih2 =>
+  intro Γ' cc cc'
+  apply Judgment.allk
+  apply ih1 Γ' cc c1
+  apply ih2 Γ' cc c2
+case _ κ1' κ2' _ _ _ _ _ jk1 jk2 ck1 ck2 c1 c2 ihk1 ihk2 ih1 ih2 =>
+  intro Γ' k' cc h1 h2 jk2' cc'; -- k' = κ2'
+  have ihk1' := ihk1 Γ' (κ1' -k> κ2') cc; simp at ihk1';
+  have ihk2' := ihk2 Γ' (k') cc; simp at ihk2';
+  -- have ih1' := ih1 Γ' (κ1' -k> k'); simp at ih1';
+  -- have ih1'' := ih1' cc (HsJudgment.arrowk jk1 jk2);
+  -- have ih2' := ih2 Γ' κ1'; simp at ih2';
+  apply Judgment.appk;
+  case _ => sorry
+  case _ => sorry
+  apply κ1'
+case _ => sorry
+case _ => sorry
+case _ => sorry
+case _ => sorry
+case _ => sorry
+case _ => sorry
+case _ =>
+  intro Γ' τ' cc c1 jk ck;
+  sorry
+
+case _ =>
+  intro Γ' τ' cc c4 j1 c1
+  apply Judgment.letterm
+  sorry
+  sorry
+  sorry
+  sorry
+case _ =>
+  intro Γ' τ' cc c5 j1 c1
+  apply Judgment.ite;
+  sorry
+  sorry
+  sorry
+  sorry
+  sorry
+  sorry
+  sorry
+  sorry
+  sorry
+  sorry
+  sorry
+  sorry
+  sorry
 
 
 -- case _ => intros; apply Judgment.wfnil;
