Hs/Metatheory/Substitution.lean
@@ -1,0 +1,433 @@
+import Hs.HsTerm
+import Hs.HsJudgment
+import SystemFD.Ctx
+import Hs.Metatheory.TypeMatch
+import Hs.Metatheory.Weaken
+
+set_option maxHeartbeats 500000
+
+def lift_subst_replace (A : Frame HsTerm) :
+  ⊢s (A.apply σ :: Δ) ->
+  (∀ n t T, σ n = .su t -> .some T = (Γ d@ n).get_type -> Δ ⊢s t : ([σ]T)) ->
+  (∀ n t T, ^σ n = .su t -> .some T = ((A::Γ) d@ n).get_type -> (A.apply σ :: Δ) ⊢s t : ([^σ]T))
+:= by sorry
+-- intro j h1 n t T h2 h3
+-- cases n <;> simp at *
+-- case _ n =>
+--   unfold Subst.compose at h2; simp at h2
+--   generalize ydef : σ n = y at *
+--   cases y <;> simp at h2
+--   case _ t' =>
+--     subst h2
+--     have lem : Option.map ([P]·) (some T) = (Γ d@ n).get_type := by
+--       rw [h3]; simp; unfold Function.comp; simp
+--     simp at lem
+--     replace h1 := h1 n t' ([P]T) ydef lem
+--     have lem2 : ∃ T', T = [S]T' := by
+--       generalize wdef : (Γ d@ n).get_type = w at *
+--       cases w
+--       case _ => cases lem
+--       case _ T' => simp at h3; exists T'
+--     have lem3 : [S ⊙ σ ⊙ P]T = [^σ]T := by
+--       cases lem2; case _ T' lem2 =>
+--       subst lem2; simp; rw [<-Subst.assoc]
+--       rw [Subst.P_after_S]; simp
+--     have lem4 := weaken j h1; simp at lem4
+--     rw [lem3] at lem4; simp at lem4
+--     apply lem4
+
+@[simp]
+abbrev idx_subst (σ : Subst HsTerm) : HsJudgmentArgs v -> HsJudgmentArgs v :=
+  match v with
+  | .prf => λ (t, A) => ([σ]t, [σ]A)
+  | .wf => λ () => ()
+
+def subst :
+  (∀ n y, σ n = .re y -> (Γ d@ n).apply σ = Δ d@ y) ->
+  (∀ n t T, σ n = .su t -> .some T = (Γ d@ n).get_type -> Δ ⊢s t : ([σ]T)) ->
+  (∀ n, Γ.is_stable n -> ∃ y, σ n = .re y) ->
+  HsJudgment v Γ idx ->
+  ⊢s Δ ->
+  HsJudgment v Δ (idx_subst σ idx)
+:= by sorry
+-- intro h1 h2 h3 j wf
+-- induction j generalizing Δ σ
+-- any_goals (solve | apply wf)
+-- case letterm A t b T j1 j2 j3 j4 ih1 ih2 ih3 ih4 =>
+--   simp at *
+--   have lem1 := ih1 h1 h2 h3 wf
+--   have lem2 := ih2 h1 h2 h3 wf
+--   have lem3 : ⊢s ((Frame.term A t).apply σ :: Δ) := by
+--     apply Judgment.wfterm lem1 lem2 wf
+--   replace ih3 := @ih3 (^σ) ((Frame.term A t).apply σ :: Δ)
+--     (lift_subst_rename (Frame.term A t) h1)
+--     (lift_subst_replace (Frame.term A t) lem3 h2)
+--     (lift_subst_stable (Frame.term A t) h3)
+--     lem3
+--   simp at ih3
+--   apply Judgment.letterm lem1 lem2
+--   simp; apply ih3; apply ih4 h1 h2 h3 wf
+-- case ax ih =>
+--   simp at *
+--   apply Judgment.ax wf
+-- case var Γ x T j1 j2 ih =>
+--   simp at *
+--   generalize zdef : σ x = z at *
+--   cases z <;> simp
+--   case _ y =>
+--     constructor; apply wf; rw [<-h1 _ _ zdef]
+--     rw [Frame.get_type_apply_commute, <-j2]; simp
+--   case _ t => apply h2 x _ _ zdef j2
+-- case _ ih1 ih2 =>
+--   simp at *
+--   replace ih1 := ih1 h1 h2 h3 wf
+--   replace ih2 := ih2 h1 h2 h3 wf
+--   apply Judgment.allk ih1 ih2
+-- case _ Γ A B j1 j2 ih1 ih2 =>
+--   simp at *
+--   have lem := ih1 h1 h2 h3 wf
+--   have lem2 : ⊢s ((Frame.kind A).apply σ :: Δ) := by
+--     apply Judgment.wfkind lem wf
+--   replace ih2 := @ih2 (^σ) ((Frame.kind A).apply σ :: Δ)
+--     (lift_subst_rename (Frame.kind A) h1)
+--     (lift_subst_replace (Frame.kind A) lem2 h2)
+--     (lift_subst_stable (Frame.kind A) h3)
+--     lem2
+--   simp at ih2
+--   constructor; apply lem; apply ih2
+-- case _ A _ _ _ ih1 ih2 =>
+--   simp at *
+--   replace ih1 := ih1 h1 h2 h3 wf
+--   have lem2 : ⊢s ((Frame.empty).apply σ :: Δ) := by
+--     constructor; assumption
+--   replace ih2 := @ih2 (^σ) ((Frame.empty).apply σ :: Δ)
+--     (lift_subst_rename (Frame.empty) h1)
+--     (lift_subst_replace (Frame.empty) lem2 h2)
+--     (lift_subst_stable (Frame.empty) h3)
+--     lem2
+--   simp at ih2
+--   apply Judgment.arrow ih1 ih2
+-- case _ ih1 ih2 =>
+--   simp at *
+--   replace ih1 := ih1 h1 h2 h3 wf
+--   replace ih2 := ih2 h1 h2 h3 wf
+--   apply Judgment.appk ih1 ih2
+-- case _ ih1 ih2 ih3 =>
+--   simp at *
+--   replace ih1 := ih1 h1 h2 h3 wf
+--   replace ih2 := ih2 h1 h2 h3 wf
+--   replace ih3 := ih3 h1 h2 h3 wf
+--   apply Judgment.eq ih1 ih2 ih3
+-- case ite Γ p A s R i B T e j1 j2 j3 j4 j5 j6 j7 j8 j9 j10 ih1 ih2 ih3 ih4 ih5 ih6 =>
+--   replace ih1 := ih1 h1 h2 h3 wf
+--   replace ih2 := ih2 h1 h2 h3 wf
+--   replace ih3 := ih3 h1 h2 h3 wf
+--   replace ih4 := ih4 h1 h2 h3 wf
+--   replace ih5 := ih5 h1 h2 h3 wf
+--   replace ih6 := ih6 h1 h2 h3 wf
+--   replace j7 := stable_type_match_subst h1 h3 j7
+--   replace j8 := prefix_type_match_subst h1 h3 j8
+--   apply Judgment.ite ih1 ih2 ih3 ih4 _ _ j7 j8 ih5 ih6
+--   case _ =>
+--     apply valid_head_variable_subst Γ.is_ctor Δ.is_ctor _ j5
+--     intro n h
+--     have lem : Γ.is_stable n := by
+--       apply Frame.is_ctor_implies_is_stable h
+--     replace h3 := h3 n lem
+--     cases h3; case _ y h3 =>
+--     apply Exists.intro y; apply And.intro h3
+--     replace h1 := h1 _ _ h3
+--     simp at h; simp; rw [<-@Frame.is_ctor_stable _ _ σ _] at h
+--     rw [h1] at h; apply h
+--   case _ =>
+--     apply valid_head_variable_subst Γ.is_datatype Δ.is_datatype _ j6
+--     intro n h
+--     have lem : Γ.is_stable n := by
+--       apply Frame.is_datatype_implies_is_stable h
+--     replace h3 := h3 n lem
+--     cases h3; case _ y h3 =>
+--     apply Exists.intro y; apply And.intro h3
+--     replace h1 := h1 _ _ h3
+--     simp at h; simp; rw [<-@Frame.is_datatype_stable _ _ σ _] at h
+--     rw [h1] at h; apply h
+-- case guard Γ p A s R t B T j1 j2 j3 j4 j5 j6 j7 j8 j9 ih1 ih2 ih3 ih4 ih5 =>
+--   replace ih1 := ih1 h1 h2 h3 wf
+--   replace ih2 := ih2 h1 h2 h3 wf
+--   replace ih3 := ih3 h1 h2 h3 wf
+--   replace ih4 := ih4 h1 h2 h3 wf
+--   replace ih5 := ih5 h1 h2 h3 wf
+--   replace j7 := stable_type_match_subst h1 h3 j7
+--   replace j8 := prefix_type_match_subst h1 h3 j8
+--   apply Judgment.guard ih1 ih2 ih3 ih4 _ _ j7 j8 ih5
+--   case _ =>
+--     apply valid_head_variable_subst Γ.is_insttype Δ.is_insttype _ j5
+--     intro n h
+--     have lem : Γ.is_stable n := by
+--       apply Frame.is_insttype_implies_is_stable h
+--     replace h3 := h3 n lem
+--     cases h3; case _ y h3 =>
+--     apply Exists.intro y; apply And.intro h3
+--     replace h1 := h1 _ _ h3
+--     simp at h; simp; rw [<-@Frame.is_insttype_stable _ _ σ _] at h
+--     rw [h1] at h; apply h
+--   case _ =>
+--     apply valid_head_variable_subst Γ.is_opent Δ.is_opent _ j6
+--     intro n h
+--     have lem : Γ.is_stable n := by
+--       apply Frame.is_opent_implies_is_stable h
+--     replace h3 := h3 n lem
+--     cases h3; case _ y h3 =>
+--     apply Exists.intro y; apply And.intro h3
+--     replace h1 := h1 _ _ h3
+--     simp at h; simp; rw [<-@Frame.is_opent_stable _ _ σ _] at h
+--     rw [h1] at h; apply h
+-- case _ Γ A t B j1 j2 j3 ih1 ih2 ih3 =>
+--   simp at *
+--   replace ih1 := ih1 h1 h2 h3 wf
+--   replace ih3 := ih3 h1 h2 h3 wf
+--   have lem2 : ⊢s ((Frame.type A).apply σ :: Δ) := by
+--     constructor; assumption; assumption
+--   replace ih2 := @ih2 (^σ) ((Frame.type A).apply σ :: Δ)
+--     (lift_subst_rename (Frame.type A) h1)
+--     (lift_subst_replace (Frame.type A) lem2 h2)
+--     (lift_subst_stable (Frame.type A) h3)
+--     lem2
+--   simp at ih2
+--   apply Judgment.lam ih1 ih2 ih3
+-- case _ ih1 ih2 =>
+--   simp at *
+--   replace ih1 := ih1 h1 h2 h3 wf
+--   replace ih2 := ih2 h1 h2 h3 wf
+--   apply Judgment.app ih1 ih2; simp [*]
+-- case _ Γ A t B j1 j2 j3 ih1 ih2 ih3 =>
+--   simp at *
+--   replace ih1 := ih1 h1 h2 h3 wf
+--   replace ih3 := ih3 h1 h2 h3 wf
+--   have lem2 : ⊢s ((Frame.kind A).apply σ :: Δ) := by
+--     apply Judgment.wfkind ih1 wf
+--   replace ih2 := @ih2 (^σ) ((Frame.kind A).apply σ :: Δ)
+--     (lift_subst_rename (Frame.kind A) h1)
+--     (lift_subst_replace (Frame.kind A) lem2 h2)
+--     (lift_subst_stable (Frame.kind A) h3)
+--     lem2
+--   simp at ih2
+--   apply Judgment.lamt ih1 ih2 ih3
+-- case _ ih1 ih2 =>
+--   simp at *
+--   replace ih1 := ih1 h1 h2 h3 wf
+--   replace ih2 := ih2 h1 h2 h3 wf
+--   apply Judgment.appt ih1 ih2; simp [*]
+-- case _ ih1 ih2 =>
+--   simp at *
+--   replace ih1 := ih1 h1 h2 h3 wf
+--   replace ih2 := ih2 h1 h2 h3 wf
+--   apply Judgment.cast ih1 ih2
+-- case _ ih1 ih2 =>
+--   simp at *
+--   replace ih1 := ih1 h1 h2 h3 wf
+--   replace ih2 := ih2 h1 h2 h3 wf
+--   apply Judgment.refl ih1 ih2
+-- case _ ih =>
+--   simp at *
+--   replace ih := ih h1 h2 h3 wf
+--   apply Judgment.sym ih
+-- case _ ih1 ih2 =>
+--   simp at *
+--   replace ih1 := ih1 h1 h2 h3 wf
+--   replace ih2 := ih2 h1 h2 h3 wf
+--   apply Judgment.seq ih1 ih2
+-- case _ ih1 ih2 ih3 ih4 ih5 ih6 =>
+--   simp at *
+--   replace ih1 := ih1 h1 h2 h3 wf
+--   replace ih2 := ih2 h1 h2 h3 wf
+--   replace ih3 := ih3 h1 h2 h3 wf
+--   replace ih4 := ih4 h1 h2 h3 wf
+--   replace ih5 := ih5 h1 h2 h3 wf
+--   replace ih6 := ih6 h1 h2 h3 wf
+--   apply Judgment.appc ih1 ih2 ih3 ih4 ih5 ih6
+-- case _ A B _ _ _ _ _ _ _ _ _ _ ih1 ih2 ih3 ih4 ih5 ih6 =>
+--   simp at *
+--   replace ih1 := ih1 h1 h2 h3 wf
+--   replace ih2 := ih2 h1 h2 h3 wf
+--   replace ih3 := ih3 h1 h2 h3 wf
+--   have lem1 : ⊢s ((Frame.empty).apply σ :: Δ) := by constructor; assumption;
+--   replace ih4 := @ih4 (^σ) ((Frame.empty).apply σ :: Δ)
+--     (lift_subst_rename (Frame.empty) h1)
+--     (lift_subst_replace (Frame.empty) lem1 h2)
+--     (lift_subst_stable (Frame.empty) h3)
+--     lem1
+--   simp at ih4
+--   replace ih5 := @ih5 (^σ) ((Frame.empty).apply σ :: Δ)
+--     (lift_subst_rename (Frame.empty) h1)
+--     (lift_subst_replace (Frame.empty) lem1 h2)
+--     (lift_subst_stable (Frame.empty) h3)
+--     lem1
+--   simp at ih5
+--   replace ih6 := @ih6 (^σ) ((Frame.empty).apply σ :: Δ)
+--     (lift_subst_rename (Frame.empty) h1)
+--     (lift_subst_replace (Frame.empty) lem1 h2)
+--     (lift_subst_stable (Frame.empty) h3)
+--     lem1
+--   simp at ih6
+--   apply Judgment.arrowc ih1 ih2 ih3 ih4 ih5 ih6
+-- case _ ih1 ih2 ih3 =>
+--   simp at *
+--   replace ih1 := ih1 h1 h2 h3 wf
+--   replace ih2 := ih2 h1 h2 h3 wf
+--   replace ih3 := ih3 h1 h2 h3 wf
+--   apply Judgment.fst ih1 ih2 ih3
+-- case _ ih1 ih2 ih3 ih4 =>
+--   simp at *
+--   replace ih1 := ih1 h1 h2 h3 wf
+--   replace ih2 := ih2 h1 h2 h3 wf
+--   replace ih3 := ih3 h1 h2 h3 wf
+--   replace ih4 := ih4 h1 h2 h3 wf
+--   apply Judgment.snd ih1 ih2 ih3 ih4
+-- case _ Γ K A B t j1 j2 j3 ih1 ih2 ih3 =>
+--   simp at *
+--   replace ih1 := ih1 h1 h2 h3 wf
+--   replace ih2 := ih2 h1 h2 h3 wf
+--   have lem2 : ⊢s ((Frame.kind K).apply σ :: Δ) := by
+--     cases ih1; case _ ih1 _ =>
+--       apply Judgment.wfkind ih1 wf
+--   replace ih3 := @ih3 (^σ) ((Frame.kind K).apply σ :: Δ)
+--     (lift_subst_rename (Frame.kind K) h1)
+--     (lift_subst_replace (Frame.kind K) lem2 h2)
+--     (lift_subst_stable (Frame.kind K) h3)
+--     lem2
+--   simp at ih3
+--   apply Judgment.allc ih1 ih2 ih3
+-- case _ ih1 ih2 ih3 ih4 =>
+--   simp at *
+--   replace ih1 := ih1 h1 h2 h3 wf
+--   replace ih2 := ih2 h1 h2 h3 wf
+--   replace ih3 := ih3 h1 h2 h3 wf
+--   replace ih4 := ih4 h1 h2 h3 wf
+--   apply Judgment.apptc ih1 ih2 ih3 ih4
+--   simp [*]; simp [*]
+
+def beta_empty t :
+  (.empty::Γ) ⊢s b : B ->
+  Γ ⊢s (b β[t]) : (B β[t])
+:= by sorry
+-- intro j
+-- have lem : ⊢s Γ := by
+--   have lem := hs_judgment_ctx_wf .prf j
+--   cases lem;
+-- apply @subst (.su t :: I) (.empty::Γ) Γ _ _ _ _ _ j
+-- apply lem
+-- case _ =>
+--   intro n y h1
+--   cases n <;> simp at *; subst h1
+--   case _ n =>
+--     rw [Frame.apply_compose]; simp
+-- case _ =>
+--   intro n s T h1 h2
+--   cases n <;> simp at *; subst h1
+--   injection h2
+-- case _ =>
+--   intro n h1
+--   cases n <;> simp at *
+--   rw [Frame.is_stable_stable] at h1
+--   unfold Frame.is_stable at h1
+--   simp at h1
+
+def beta_type :
+  (.type A::Γ) ⊢s b : B ->
+  Γ ⊢s t : A ->
+  Γ ⊢s (b β[t]) : (B β[t])
+:= by sorry
+-- intro j1 j2
+-- apply @subst (.su t :: I) (.type A::Γ) Γ _ _ _ _ _ j1
+-- apply judgment_ctx_wf j2
+-- case _ =>
+--   intro n y h1
+--   cases n <;> simp at *; subst h1
+--   case _ n =>
+--     rw [Frame.apply_compose]; simp
+-- case _ =>
+--   intro n s T h1 h2
+--   cases n <;> simp at *; subst h1
+--   injection h2 with e; subst e; simp
+--   apply j2
+-- case _ =>
+--   intro n h1
+--   cases n <;> simp at *
+--   rw [Frame.is_stable_stable] at h1
+--   unfold Frame.is_stable at h1
+--   simp at h1
+
+def beta_kind :
+  (.kind A::Γ) ⊢s b : B ->
+  Γ ⊢s t : A ->
+  Γ ⊢s (b β[t]) : (B β[t])
+:= by sorry
+-- intro j1 j2
+-- apply @subst (.su t :: I) (.kind A::Γ) Γ _ _ _ _ _ j1
+-- apply judgment_ctx_wf j2
+-- case _ =>
+--   intro n y h1
+--   cases n <;> simp at *; subst h1
+--   case _ n =>
+--     rw [Frame.apply_compose]; simp
+-- case _ =>
+--   intro n s T h1 h2
+--   cases n <;> simp at *; subst h1
+--   injection h2 with e; subst e; simp
+--   apply j2
+-- case _ =>
+--   intro n h1
+--   cases n <;> simp at *
+--   rw [Frame.is_stable_stable] at h1
+--   unfold Frame.is_stable at h1
+--   simp at h1
+
+def beta_term :
+  (.term A t::Γ) ⊢s b : B ->
+  Γ ⊢s t : A ->
+  Γ ⊢s (b β[t]) : (B β[t])
+:= by sorry
+-- intro j1 j2
+-- apply @subst (.su t :: I) (.term A t::Γ) Γ _ _ _ _ _ j1
+-- apply judgment_ctx_wf j2
+-- case _ =>
+--   intro n y h1
+--   cases n <;> simp at *; subst h1
+--   case _ n =>
+--     rw [Frame.apply_compose]; simp
+-- case _ =>
+--   intro n s T h1 h2
+--   cases n <;> simp at *; subst h1
+--   injection h2 with e; subst e; simp
+--   apply j2
+-- case _ =>
+--   intro n h1
+--   cases n <;> simp at *
+--   rw [Frame.is_stable_stable] at h1
+--   unfold Frame.is_stable at h1
+--   simp at h1
+
+def beta_openm :
+  (.openm A::Γ) ⊢s b : B ->
+  Γ ⊢s t : A ->
+  Γ ⊢s (b β[t]) : (B β[t])
+:= by sorry
+-- intro j1 j2
+-- apply @subst (.su t :: I) (.openm A::Γ) Γ _ _ _ _ _ j1
+-- apply judgment_ctx_wf j2
+-- case _ =>
+--   intro n y h1
+--   cases n <;> simp at *; subst h1
+--   case _ n =>
+--     rw [Frame.apply_compose]; simp
+-- case _ =>
+--   intro n s T h1 h2
+--   cases n <;> simp at *; subst h1
+--   injection h2 with e; subst e; simp
+--   apply j2
+-- case _ =>
+--   intro n h1
+--   cases n <;> simp at *
+--   rw [Frame.is_stable_stable] at h1
+--   unfold Frame.is_stable at h1
+--   simp at h1
